prove Row_insert_body in a rather ugly way

examples/sbf/verif.v
@@ -56,108 +56,11 @@ Definition Row_spec : func_spec :=
            if (op =? CLEAR)%Z then row_clear r i else
            r)]))).
 
-(* Program:
-  action act_insert() {
-      rw = regact_insert.execute(index);
-  }
-*)
-
-Definition Row_insert_spec : func_spec :=
-  WITH (* p *),
-    PATH p
-    MOD (Some [["rw"]]) [p]
-    WITH (r : row) (i : Z)
-      (_ : 0 <= i < Zlength r),
-      PRE
-        (ARG []
-        (MEM [(["index"], eval_val_to_sval (ValBaseBit (P4Arith.to_lbool 16%N i)))]
-        (EXT [row_repr p r])))
-      POST
-        (ARG_RET [] ValBaseNull
-        (MEM [(["rw"], eval_val_to_sval (ValBaseBit (P4Arith.to_lbool 8%N 1)))]
-        (EXT [row_repr p (row_insert r i)]))).
-
 Definition num_cells := 65536.
-
-Definition Row_regact_insert_execute_spec : func_spec :=
-  WITH (* p *),
-    PATH p ++ ["regact_insert"]
-    MOD None [p ++ ["reg_row"]]
-    WITH (r : row) (i : Z)
-      (H_r : Zlength r = num_cells)
-      (H_i : 0 <= i < num_cells),
-      PRE
-        (ARG [eval_val_to_sval (ValBaseBit (P4Arith.to_lbool 16%N i))]
-        (MEM []
-        (EXT [ExtPred.singleton (p ++ ["reg_row"]) (Tofino.ObjRegister (map bool_to_val r))])))
-      POST
-        (ARG_RET [] (eval_val_to_sval (ValBaseBit (P4Arith.to_lbool 8%N 1)))
-        (MEM []
-        (EXT [ExtPred.singleton (p ++ ["reg_row"])
-            (Tofino.ObjRegister (upd_Znth i (map bool_to_val r) (bool_to_val true)))]))).
 
 Definition dummy_fundef : @fundef Info := FExternal "" "".
 Opaque dummy_fundef.
 Definition execute_fundef : @fundef Info := FExternal "RegisterAction" "execute".
-
-Definition Row_regact_insert_apply_fundef := Eval compute -[am_ge] in
-  (force Tofino.EnvPin (PathMap.get (p ++ ["regact_insert"; "apply"]) (ge_ext ge))).
-
-Definition Row_regact_insert_apply :=
-  FInternal [(["apply"; "value"], InOut); (["apply"; "rv"], Out)]
-    (BlockCons
-       (MkStatement NoInfo
-          (StatVariable (TypTypeName {| P4String.tags := NoInfo; str := "bf2_value_t" |})
-             {| P4String.tags := NoInfo; str := "rv" |} None (LInstance ["rv"])) StmUnit)
-       (BlockCons
-          (MkStatement NoInfo
-             (StatAssignment
-                (MkExpression NoInfo
-                   (ExpName (BareName {| P4String.tags := NoInfo; str := "value" |})
-                      (LInstance ["apply"; "value"]))
-                   (TypTypeName {| P4String.tags := NoInfo; str := "bf2_value_t" |}) InOut)
-                (MkExpression NoInfo
-                   (ExpInt
-                      {| tags := NoInfo; value := 1; width_signed := Some (8%N, false) |})
-                   (TypBit 8) Directionless)) StmUnit)
-          (BlockCons
-             (MkStatement NoInfo
-                (StatAssignment
-                   (MkExpression NoInfo
-                      (ExpName (BareName {| P4String.tags := NoInfo; str := "rv" |})
-                         (LInstance ["apply"; "rv"]))
-                      (TypTypeName {| P4String.tags := NoInfo; str := "bf2_value_t" |}) Out)
-                   (MkExpression NoInfo
-                      (ExpInt
-                         {| tags := NoInfo; value := 1; width_signed := Some (8%N, false) |})
-                      (TypBit 8) Directionless)) StmUnit) (BlockEmpty NoInfo)))).
-
-Definition Row_regact_insert_apply_spec : func_spec :=
-  WITH,
-    PATH (p ++ ["regact_insert"])
-    MOD None []
-    WITH,
-      PRE
-        (ARG [ValBaseBit (repeat None 8)]
-        (MEM []
-        (EXT [])))
-      POST
-        (ARG_RET [ValBaseBit (P4Arith.to_loptbool 8%N 1);
-                  ValBaseBit (P4Arith.to_loptbool 8%N 1)]
-           ValBaseNull
-        (MEM []
-        (EXT []))).
-
-Lemma Row_regact_insert_apply_body :
-  fundef_satisfies_spec am_ge Row_regact_insert_apply nil Row_regact_insert_apply_spec.
-Proof.
-  start_function.
-  step.
-  step.
-  step.
-  step.
-  entailer.
-Qed.
 
 (* This is the general form of RegisterAction's apply method's spec that we support.
   We expecct this is general enough for all practical application. We don't support
@@ -414,198 +317,37 @@ Proof.
   }
 Admitted.
 
-(* So the problem here is that, we need to define a rule for execute.
-  And, should the ge constraint in spec for read and write be on the path quantifier? *)
+Definition Row_regact_insert_apply_sem := Eval compute -[am_ge] in
+  (force Tofino.EnvPin (PathMap.get (p ++ ["regact_insert"; "apply"]) (ge_ext ge))).
 
-(* Currently we have two problem. One is to use abstract method spec to prove execute.
-The other is to find a way to prevent unfolding Extern typeclass in the computation of ge. *)
+Definition Row_regact_insert_apply_fd :=
+  ltac : (
+    let sem := eval unfold Row_regact_insert_apply_sem in Row_regact_insert_apply_sem in
+    match sem with
+    | Tofino.EnvAbsMet (exec_abstract_method ?ge ?p ?fd) =>
+        exact fd
+    end).
 
-Lemma Row_regact_insert_execute_body :
-  fundef_satisfies_spec ge execute_fundef nil Row_regact_insert_execute_spec.
+Definition Row_regact_insert_apply_spec : func_spec :=
+  RegisterAction_apply_spec (p ++ ["regact_insert"]) 8 (fun _ => 1)
+    (fun _ => ValBaseBit (P4Arith.to_loptbool 8%N 1)).
+
+Lemma Row_regact_insert_apply_body :
+  fundef_satisfies_spec am_ge Row_regact_insert_apply_fd nil Row_regact_insert_apply_spec.
 Proof.
-Admitted.
-(*   split.
-  2 : {
-    unfold func_modifies; intros.
-    inv H.
-    inv H5. inv H. compute in H0. inv H0.
-    compute in H3; inv H3.
-    destruct (-1 <? index) eqn:?.
-    2 : {
-      simpl in H8. destruct H8; subst.
-      apply modifies_refl.
-    }
-    destruct (index <? 65536) eqn:?.
-    2 : {
-      simpl in H8. destruct H8; subst.
-      apply modifies_refl.
-    }
-    simpl in H8. destruct H8; subst.
-    compute - [am_ge] in H1. inv H1.
-    eapply modifies_trans.
-    { eapply modifies_incl.
-      assert (modifies None [] (m, es) (m, s')). {
-        change
-          (exec_abstract_method (tags_t := Info) (target := target) am_ge (p ++ ["regact_insert"])
-            Row_regact_insert_apply
-            es [old_value] s' [new_value; retv] SReturnNull)
-          in H7.
-        inv H7.
-        split.
-        { constructor. }
-        { simpl.
-          apply Row_regact_insert_apply_body in H1.
-          apply H1.
-        }
-      }
-      eassumption.
-      solve_modifies.
-      solve_modifies.
-    }
-    eapply modifies_set_ext with (st := (m, s')).
-    auto.
-  }
-  repeat lazymatch goal with
-  | |- fundef_satisfies_hoare _ _ _ _ (fsh_bind (fun x => _)) =>
-    let x := fresh x in intro x
-  end;
-  unfold fundef_satisfies_hoare.
-  unfold hoare_func; intros.
-  inv H0. inv H6.
-  cbn - [ge] in H0.
-  inv H0.
-  compute in H1. inv H1. (* get reg from ge *)
-  compute in H4. inv H4. (* get (w, size) from ge *)
-  destruct H as [? [_ ?]].
-  assert (index = i). {
-    clear -H_i H H3 H6.
-    unfold arg_denote, arg_satisfies in H.
-    remember (eval_val_to_sval (ValBaseBit (P4Arith.to_lbool 16 i))) as x in H.
-    inv H. inv H5.
-    inv H3. clear H7.
-    assert (ValBaseBit indexb = (ValBaseBit (P4Arith.to_lbool 16 i))). {
-      eapply exec_val_eq.
-      eapply exec_val_sym with eq.
-      { clear; auto. }
-      assert (val_to_sval
-          (ValBaseBit (P4Arith.to_lbool 16 i))
-          (eval_val_to_sval (ValBaseBit (P4Arith.to_lbool 16 i)))). {
-        eapply exec_val_sym with strict_read_ndetbit.
-        2 : eapply sval_to_val_eval_val_to_sval.
-        { clear; sauto. }
-        { clear; sauto. }
-      }
-      eapply exec_val_trans with (f := read_detbit);
-        [ | eapply exec_val_trans; [ | eassumption | eassumption] | eassumption ].
-      { unfold rel_trans; clear; sauto. }
-      { unfold rel_trans; clear; sauto. }
-    }
-    inv H.
-    rewrite P4Arith.bit_from_to_bool in H6.
-    inv H6.
-    apply Z.mod_small; assumption.
-  }
-  clear H H3 H6.
-  subst.
-  destruct (-1 <? i) eqn:Heqb; only 2 : lia. clear Heqb.
-  destruct (i <? 65536) eqn:Heqb; only 2 : (unfold num_cells in H_i; lia). clear Heqb.
-  compute -[target am_ge] in H2. inv H2.
-  change
-    (exec_abstract_method (tags_t := Info) (target := target) am_ge (p ++ ["regact_insert"])
-      Row_regact_insert_apply
-      es [old_value] s' [new_value; retv] SReturnNull)
-    in H8.
-  simpl in H7. destruct H9. subst.
-  assert (content = map bool_to_val r). {
-    clear -H0 H5.
-    inv H0.
-    simpl in H.
-    congruence.
-  }
-  clear H0.
-  subst.
-  assert (content' = map bool_to_val r). {
-    clear -H H5 H8.
-    inv H8.
-    apply (Row_regact_insert_apply_body) in H1.
-    destruct H1.
-    assert (PathMap.get ["pipe"; "ingress"; "bf2_ds"; "win_1"; "row_1"; "reg_row"] s'
-        = PathMap.get ["pipe"; "ingress"; "bf2_ds"; "win_1"; "row_1"; "reg_row"] es). {
-      symmetry.
-      apply H3.
-      auto.
-    }
-    rewrite H4 in H.
-    change (@extern_object Info (@Expression Info) (@extern_sem Info (@Expression Info) target))
-      with (@Tofino.object Info (@Expression Info)) in H.
-    rewrite H5 in H.
-    congruence.
-  }
-  clear H H5.
-  subst.
-  rewrite Znth_map in H8 by list_solve.
-  assert (new_value = ValBaseBit (P4Arith.to_lbool 8 1)
-      /\ retv = ValBaseBit (P4Arith.to_lbool 8 1)). {
-    clear -H8.
-    inv H8.
-    apply (proj1 Row_regact_insert_apply_body) in H0.
-    2 : {
-      split.
-      2 : { split; constructor. }
-      inv H. inv H4. inv H6.
-      do 9 lazymatch goal with
-      | H : Forall2 read_detbit _ _ |- _ =>
-          inv H
-      end.
-      do 8 lazymatch goal with
-      | H : read_detbit _ _ |- _ =>
-          inv H
-      end.
-      repeat constructor.
-    }
-    destruct H0.
-    inv H0. inv H7. inv H8.
-    assert (forall width value sv,
-      sval_refine (ValBaseBit (P4Arith.to_loptbool width value)) sv ->
-      sv = (ValBaseBit (P4Arith.to_loptbool width value))
-    ) as sval_refine_bit_to_loptbool by admit.
-    apply sval_refine_bit_to_loptbool in H4, H5; subst.
-    inv H1. inv H7. clear H8.
-    assert (forall width value v,
-      sval_to_val read_ndetbit (ValBaseBit (P4Arith.to_loptbool width value)) v ->
-      v = (ValBaseBit (P4Arith.to_lbool width value))
-    ) as sval_to_val_bit_to_loptbool by admit.
-    apply sval_to_val_bit_to_loptbool in H4, H5; subst.
-    auto.
-  }
-  clear H8.
-  destruct H; subst.
-  simpl.
-  split.
-  { inv H12. constructor. }
-  clear H12.
-  split.
-  { unfold ret_denote, ret_satisfies.
-    intros.
-    assert (forall width value sv,
-      val_to_sval (ValBaseBit (P4Arith.to_lbool width value)) sv ->
-      sv = (ValBaseBit (P4Arith.to_loptbool width value))
-    ) as val_to_sval_bit_to_lbool by admit.
-    apply val_to_sval_bit_to_lbool in H. subst.
-    repeat constructor.
-  }
-  split.
-  { constructor. }
-  { constructor.
-    2 : constructor.
-    simpl.
-    rewrite PathMap.get_set_same.
-    auto.
-  }
-Admitted. *)
+  start_function.
+  step.
+  step.
+  step.
+  step.
+  entailer.
+Qed.
+
+Program Definition Row_regact_insert_execute_body :=
+  RegisterAction_execute_body _ 16%N 8%N num_cells (p ++ ["reg_row"]) eq_refl eq_refl ltac:(abstract (unfold num_cells; lia))
+    Row_regact_insert_apply_fd (fun _ => 1) (fun _ => ValBaseBit (P4Arith.to_loptbool 8%N 1)) eq_refl Row_regact_insert_apply_body.
 
 #[local] Hint Extern 5 (func_modifies _ _ _ _ _) => (apply Row_regact_insert_execute_body) : func_specs.
-(* #[local] Hint Extern 1 (list P4Type) => (exact (@nil _)) : func_specs. *)
 
 Axiom Row_regact_query_execute_modifies :
   func_modifies ge (p ++ ["regact_query"]) (FExternal "RegisterAction" "execute") None [].
@@ -625,6 +367,28 @@ Definition NoAction_fundef : @fundef Info := Eval compute in
 Definition Row_insert_fundef := Eval compute in
   force dummy_fundef (PathMap.get ["Bf2BloomFilterRow"; "act_insert"] (ge_func ge)).
 
+(* Program:
+  action act_insert() {
+      rw = regact_insert.execute(index);
+  }
+*)
+
+Definition Row_insert_spec : func_spec :=
+  WITH (* p *),
+    PATH p
+    MOD (Some [["rw"]]) [p]
+    WITH (r : row) (i : Z)
+      (_ : Zlength r = num_cells)
+      (_ : 0 <= i < Zlength r),
+      PRE
+        (ARG []
+        (MEM [(["index"], eval_val_to_sval (ValBaseBit (P4Arith.to_lbool 16%N i)))]
+        (EXT [row_repr p r])))
+      POST
+        (ARG_RET [] ValBaseNull
+        (MEM [(["rw"], eval_val_to_sval (ValBaseBit (P4Arith.to_lbool 8%N 1)))]
+        (EXT [row_repr p (row_insert r i)]))).
+
 Lemma Row_insert_body :
   fundef_satisfies_spec ge Row_insert_fundef nil Row_insert_spec.
 Proof.
@@ -632,15 +396,18 @@ Proof.
   unfold row_repr, row_reg_repr.
   normalize_EXT.
   step_call Row_regact_insert_execute_body.
-  3 : { entailer. }
-  { admit. }
-  { admit. }
+  4 : { entailer. }
+  { list_solve. }
+  { list_solve. }
+  { rewrite Znth_map by list_solve.
+    split; reflexivity.
+  }
   step.
   entailer.
   f_equal.
   unfold row_insert.
   list_solve.
-Admitted.
+Qed.
 
 Definition Row_fundef := Eval compute in
   force dummy_fundef (PathMap.get ["Bf2BloomFilterRow"; "apply"] (ge_func ge)).
